skolemize

src/coding.lean
@@ -29,7 +29,7 @@ end nat
 
 
 namespace fopl
-variables {L : language.{u}} [∀ n, denumerable (L.fn n)] [∀ n, denumerable (L.pr n)]
+variables {L : language.{u}} [∀ n, encodable (L.fn n)] [∀ n, encodable (L.pr n)]
 /- inductive vecterm (L : language.{u}) : ℕ → Type u
 | nil {} : vecterm 0
 | cons   : ∀ {n : ℕ}, vecterm 1 → vecterm n → vecterm (n+1)
@@ -46,7 +46,7 @@ def vecterm.encode : ∀ {n}, vecterm L n → ℕ
 | _ (vecterm.cons a v)     := (a.encode.mkpair v.encode)
 | _ #0                     := 0
 | _ #1                     := 1
-| _ #(n+2)                   := (bit0 n) + 2
+| _ #(n+2)                 := (bit0 n) + 2
 | _ (vecterm.const c)      := (bit1 $ bit0 (encode c)) + 2
 | _ (@vecterm.app _ n f v) := (bit1 $ bit1 $ n.mkpair ((encode f).mkpair v.encode)) + 2
 
@@ -58,7 +58,7 @@ def iterate01  (L) : ∀ n, vecterm L n
 | 0     := #1
 | (n+1) := vecterm.cons #0 (iterate01 n)
 
-def of_nat_vecterm (L : language.{u}) [∀ n, denumerable (L.fn n)] : ℕ → ∀ n, vecterm L n
+def vecterm.decode (L : language.{u}) [∀ n, encodable (L.fn n)] : ℕ → ∀ n, option (vecterm L n)
 | 0     n     := iterate0 L n
 | 1     n     := iterate01 L n
 | (e+2) 0     :=
@@ -68,17 +68,19 @@ def of_nat_vecterm (L : language.{u}) [∀ n, denumerable (L.fn n)] : ℕ → �
          refine le_trans (nat.unpair_right_le _) (nat.unpair_right_le _) },
     have e.div2.div2.unpair.2.unpair.2 < e + 2 :=  nat.lt_succ_iff.mpr (le_add_right div2222),
     match e.bodd, e.div2.bodd with
-    | ff, _  := #(e.div2+2)
-    | tt, ff := vecterm.const (of_nat (L.fn 0) (e.div2.div2))
-    | tt, tt := vecterm.app (of_nat (L.fn (e.div2.div2.unpair.1 + 1)) e.div2.div2.unpair.2.unpair.1)
-      (of_nat_vecterm (e.div2.div2.unpair.2.unpair.2) e.div2.div2.unpair.1)
+    | ff, _  := some (#(e.div2+2))
+    | tt, ff := (decode (L.fn 0) (e.div2.div2)).map vecterm.const
+    | tt, tt := do
+        f ← decode (L.fn (e.div2.div2.unpair.1 + 1)) e.div2.div2.unpair.2.unpair.1,
+        v ← vecterm.decode (e.div2.div2.unpair.2.unpair.2) e.div2.div2.unpair.1,
+      vecterm.app f v
     end
 | (e+2) (n+1) := 
   have (e+2).unpair.1 < e + 2 := nat.unpair_lt (sup_eq_left.mp rfl),
   have (e+2).unpair.2 < e + 2 := nat.unpair_lt2 ((cmp_eq_lt_iff 1 (e + 2)).mp rfl),
-    vecterm.cons (of_nat_vecterm ((e+2).unpair.1) 0) (of_nat_vecterm ((e+2).unpair.2) n) 
-using_well_founded { rel_tac := λ _ _, `[exact ⟨_, measure_wf psigma.fst⟩]  }
-
+  do a ← vecterm.decode ((e+2).unpair.1) 0,
+     v ← vecterm.decode ((e+2).unpair.2) n,
+    vecterm.cons a v
 
 @[simp] private lemma iterate0_encode : ∀ n, vecterm.encode (iterate0 L n) = 0
 | 0     := rfl
@@ -88,46 +90,22 @@ using_well_founded { rel_tac := λ _ _, `[exact ⟨_, measure_wf psigma.fst⟩] 
 | 0     := rfl
 | (n+1) := by {simp[iterate01, vecterm.encode, iterate01_encode n], refl }
 
-private lemma encode_of_nat_vecterm : ∀ e n : ℕ, vecterm.encode (of_nat_vecterm L e n) = e
-| 0     n     := by simp[of_nat_vecterm, vecterm.encode, iterate0_encode]
-| 1     n     := by simp[of_nat_vecterm, vecterm.encode, iterate01_encode]
-| (e+2) 0     := 
-    have div2222 : e.div2.div2.unpair.2.unpair.2 ≤ e :=
-    by { simp[nat.div2_val], 
-         refine (le_trans _ (le_trans (nat.div_le_self (e/2) 2) (nat.div_le_self e 2))), 
-         refine le_trans (nat.unpair_right_le _) (nat.unpair_right_le _) },
-    have e.div2.div2.unpair.2.unpair.2 < e + 2 :=  nat.lt_succ_iff.mpr (le_add_right div2222),
-    have IH : _ := encode_of_nat_vecterm e.div2.div2.unpair.2.unpair.2,
-    by { suffices : (of_nat_vecterm L (e + 2) 0).encode = nat.bit e.bodd e.div2 + 2,
-         { simp[nat.bit_decomp, this] },
-         cases C₁ : e.bodd,
-         { simp [of_nat_vecterm, vecterm.encode, nat.bit, C₁] },
-         suffices : (of_nat_vecterm L (e + 2) 0).encode = nat.bit tt (nat.bit e.div2.bodd e.div2.div2) + 2,
-         { simp[nat.bit_decomp, this] },
-         cases C₂ : e.div2.bodd; simp [of_nat_vecterm, vecterm.encode, nat.bit, C₁, C₂, IH, bit1] }
-| (e+2) (n+1) :=
-    have (e+2).unpair.1 < e + 2 := nat.unpair_lt (sup_eq_left.mp rfl),
-    have (e+2).unpair.2 < e + 2 := nat.unpair_lt2 ((cmp_eq_lt_iff 1 (e + 2)).mp rfl),
-    have IH₁ : _ := encode_of_nat_vecterm (e+2).unpair.1,
-    have IH₂ : _ := encode_of_nat_vecterm (e+2).unpair.2,
-  by { simp [of_nat_vecterm, vecterm.encode, IH₁, IH₂] }
+private lemma vecterm.decode_encode : ∀ {n} (t : vecterm L n), vecterm.decode L (vecterm.encode t) n = some t
+| (n+1) (vecterm.cons a v) := by {
+    simp[vecterm.decode, vecterm.encode],
+    cases C₁ : a.encode.mkpair v.encode, simp[vecterm.decode, iterate0], simp at C₁,
+    have := vecterm.decode_encode v, }
+| _ #0                     := by {simp[vecterm.decode, vecterm.encode, iterate0], refl}
+| _ #1                     := by {simp[vecterm.decode, vecterm.encode, iterate01], refl}
+| _ #(n+2)                 := by simp[vecterm.decode, vecterm.encode]
+| _ (vecterm.const c)      := by simp[vecterm.decode, vecterm.encode]
+| _ (@vecterm.app _ n f v) := by { simp[vecterm.decode, vecterm.encode, vecterm.decode_encode v],
+      rw [nat.div2_bit1, nat.div2_bit1, nat.unpair_mkpair], simp*, refl }
 
-private lemma of_nat_vecterm_encode : ∀ {n} (t : vecterm L n), of_nat_vecterm L (vecterm.encode t) n = t
-| (n+1) (vecterm.cons a v)     := by {
-    simp[of_nat_vecterm, vecterm.encode],
-    cases C₁ : a.encode.mkpair v.encode, simp[of_nat_vecterm, iterate0], simp at C₁,
-    have := of_nat_vecterm_encode v, }
-| _ #0                     := by simp[of_nat_vecterm, vecterm.encode, iterate0]
-| _ #1                     := by simp[of_nat_vecterm, vecterm.encode, iterate01]
-| _ #(n+2)                 := by simp[of_nat_vecterm, vecterm.encode]
-| _ (vecterm.const c)      := by simp[of_nat_vecterm, vecterm.encode]
-| _ (@vecterm.app _ n f v) := by { simp[of_nat_vecterm, vecterm.encode, of_nat_vecterm_encode v],
-      rw [nat.div2_bit1, nat.div2_bit1, nat.unpair_mkpair], simp* }
+instance (n) : encodable (vecterm L n) :=
+⟨vecterm.encode, (λ e, vecterm.decode L e n), vecterm.decode_encode⟩
 
-instance (n) : denumerable (vecterm L n) :=
-mk' ⟨vecterm.encode, (λ e, of_nat_vecterm L e n),
-     of_nat_vecterm_encode,
-     (λ e, encode_of_nat_vecterm e n)⟩
+instance : encodable (term L) := ⟨vecterm.encode, (λ e, vecterm.decode L e 0), vecterm.decode_encode⟩
 
 def form.encode : form L → ℕ
 | (form.const c)      := (bit0 $ bit0 (encode c))
