src/completeness.lean
@@ -1,0 +1,115 @@
+import deduction model data.equiv.encodable.basic
+open encodable
+
+universes u
+
+namespace fopl
+variables {L : language.{u}} 
+
+inductive language_fn (L : language.{u}) : ℕ → Type u
+| sk : ∀ (p : form L), language_fn p.arity
+| old : ∀ {n}, L.fn n → language_fn n
+
+def language.skolemize (L : language) : language := ⟨language_fn L, L.pr⟩
+
+@[simp] lemma skolemize_fn : L.skolemize.fn = language_fn L := rfl
+
+def vecterm.corresp : ∀ {n}, vecterm L n → vecterm L.skolemize n
+| _ (vecterm.cons a v) := vecterm.cons a.corresp v.corresp
+| _ (#n)               := #n
+| _ (vecterm.const c)  := vecterm.const (language_fn.old c)
+| _ (vecterm.app f v)  := vecterm.app (language_fn.old f) v.corresp
+
+instance (n) : has_coe (vecterm L n) (vecterm L.skolemize n) := ⟨vecterm.corresp⟩
+
+def form.corresp : form L → form L.skolemize
+| (form.const c) := form.const c
+| (form.app p v) := form.app p v.corresp
+| (t =̇ u)        := t.corresp =̇ u.corresp
+| (p →̇ q)       := p.corresp →̇ q.corresp
+| (¬̇p)           := ¬̇p.corresp
+| (Ȧp)           := Ȧp.corresp
+
+instance : has_coe (form L) (form L.skolemize) := ⟨form.corresp⟩
+
+def normvecvar : ∀ {n}, vecterm L n
+| 0     := #0
+| (n+1) := vecterm.cons #(n+1) normvecvar
+
+namespace skolemization
+variables {L}
+
+def skterm (p : form L) : term L.skolemize :=
+begin
+  cases C : p.arity,
+  have := language_fn.sk p, simp[C] at this, exact vecterm.const this,
+  have F : L.skolemize.fn (n+1), { have := language_fn.sk p, simp[C] at this, exact this },
+  refine vecterm.app F normvecvar
+end
+
+
+inductive theory.skolemize (T : theory L) : theory (L.skolemize)
+| sk  : ∀ (p : form L), theory.skolemize (p.corresp →̇ p.corresp.ᵉ(skterm p))
+| old : ∀ {p}, T p → theory.skolemize p
+
+end skolemization
+
+end fopl
+
+namespace fopl
+variables {L : language.{u}} [encodable (form L)] (T : theory L)
+
+
+def theory.maximum_aux (T : theory L) : ℕ → theory L
+| 0     := T
+| (s+1) := let p := idecode (form L) s in
+    if (theory.maximum_aux s +{p}).consistent then theory.maximum_aux s +{p} else theory.maximum_aux s
+
+def theory.maximum  : theory L := {p | ∃ s, T.maximum_aux s p}
+
+variables {T}
+
+lemma maximum_aux_inclusion (s) : T.maximum_aux s ⊆ T.maximum := λ p h, ⟨s, h⟩
+
+lemma maximum_consistent_aux (h : T.consistent) : ∀ s, (T.maximum_aux s).consistent
+| 0 := h
+| (s+1) := by { simp[theory.maximum_aux],
+    by_cases (T.maximum_aux s +{idecode (form L) s}).consistent; simp[h, maximum_consistent_aux s] }
+
+lemma maximum_aux_ss (s) : T.maximum_aux s ⊆ T.maximum_aux (s+1) := λ p hyp_p,
+by { simp[theory.maximum_aux], by_cases C₁ : (T.maximum_aux s)+{idecode (form L) s}.consistent; simp[C₁],
+     refine theory.add.old hyp_p, refine hyp_p }
+
+theorem maximum_maximum {p} : T.maximum ⊢̇ p ∨ T.maximum ⊢̇ ¬̇p :=
+begin
+  by_cases C : (T.maximum_aux (encode p) +{p}).consistent,
+  { left, have : T.maximum_aux (encode p + 1) = (T.maximum_aux (encode p) +{p}),
+    { simp[theory.maximum_aux, C] },
+    have : T.maximum_aux (encode p + 1) ⊢̇ p,
+    { rw this, simp },
+    refine provable.inclusion this (maximum_aux_inclusion _) },
+  { right, simp[theory.consistent] at C, rcases C with ⟨r, hyp1, hyp2⟩,
+    have hyp1 : T.maximum +{p} ⊢̇ r,
+    { refine provable.inclusion hyp1 (λ h h1, _), cases h1 with _ h,
+      refine theory.add.new, refine theory.add.old (maximum_aux_inclusion _ _ h) },
+    have hyp2 : T.maximum +{p} ⊢̇ ¬̇r,
+    { refine provable.inclusion hyp2 (λ h h1, _), cases h1 with _ h,
+      refine theory.add.new, refine theory.add.old (maximum_aux_inclusion _ _ h) },
+    show T.maximum ⊢̇ ¬̇p, from provable.raa _ hyp1 hyp2 }
+end 
+
+lemma maximum_consistent (con : T.consistent) : T.maximum.consistent :=
+begin
+  simp[theory.consistent], intros p hyp A,
+  have : ∃ s, T.maximum_aux s ⊢̇ p, from provable.proof_compact maximum_aux_ss hyp, rcases this with ⟨s₁, lmm₁⟩,
+  have : ∃ s, T.maximum_aux s ⊢̇ ¬̇p, from provable.proof_compact maximum_aux_ss A, rcases this with ⟨s₂, lmm₂⟩,
+  have lmm₁ : T.maximum_aux (max s₁ s₂) ⊢̇ p, from provable.inclusion lmm₁ (ss_le maximum_aux_ss (by simp)),
+  have lmm₂ : T.maximum_aux (max s₁ s₂) ⊢̇ ¬̇p, from provable.inclusion lmm₂ (ss_le maximum_aux_ss (by simp)),
+  have : ¬(T.maximum_aux (max s₁ s₂)).consistent, simp[theory.consistent], refine ⟨p, lmm₁, lmm₂⟩,
+  exact this (maximum_consistent_aux con _)
+end
+
+def LMmodel := 𝔗[T.maximum]
+
+
+end fopl
